Wavelet/Simulation/Br.lean
@@ -17,18 +17,11 @@ namespace Wavelet.Simulation.Br
 open Wavelet.Op Wavelet.Seq Wavelet.Dataflow Wavelet.Compile
 open Relation Lemmas
 
-universe u
-variable (Op : Type u) (χ : Type u) (V S)
-variable [instArity : Arity Op] [DecidableEq χ] [instInterp : Interp Op V S]
-
-/- TODO: Fix proof performance -/
-set_option maxHeartbeats 300000
-
 theorem sim_step_br
-  {cond}
-  (hnz : m > 0 ∧ n > 0)
-  (ec ec' : Seq.Config Op χ V S m n)
-  (pc : Dataflow.Config Op (ChanName χ) V S m n)
+  [Arity Op] [DecidableEq χ] [instInterp : Interp Op V S]
+  {cond left right}
+  {ec ec' : Seq.Config Op χ V S m n}
+  {pc : Dataflow.Config Op (ChanName χ) V S m n}
   (hsim : SimR _ _ _ _ hnz ec pc)
   (hstep : Config.Step Op χ V S ec ec')
   (hbr : ec.expr = .cont (.br cond left right)) :
@@ -54,14 +47,14 @@ theorem sim_step_br
     ⟩,
   ⟩ := hsim
   have ⟨hcarryInLoop, hwf_expr, hcurrent⟩ := hcont _ hbr
-  simp [compileExpr] at hcurrent
+  simp only [compileExpr] at hcurrent
   -- Deduce some facts from `hstep`
   cases hstep with
   | step_ret hexpr | step_tail hexpr | step_op hexpr =>
     simp [hbr] at hexpr
   | step_br hexpr hcond hcondBool =>
     rename_i condVal condBool _ _ cond'
-    simp [hbr] at hexpr
+    simp only [hbr, ExprResult.cont.injEq, Expr.br.injEq] at hexpr
     have heq_cond' := hexpr.1; subst heq_cond'
     have heq_left' := hexpr.2.1; subst heq_left'
     have heq_right' := hexpr.2.2; subst heq_right'
@@ -90,21 +83,15 @@ theorem sim_step_br
       (by simp [hlive_vars, SimR.varsToChans, hcond, ← hcondName])
     have hmem_fork :
       .fork condName #v[.switch_cond condName, .merge_cond condName] ∈ pc.proc.atoms
-      := by grind
+      := by simp [hatoms, hrest, ← hcurrent]
     have hsteps₁ : Dataflow.Config.StepPlus _ _ _ _ pc _
       := Relation.TransGen.single (Dataflow.Config.Step.step_fork hmem_fork hpop_cond)
     -- Simplify pushes
     rw [push_vals_empty] at hsteps₁
     rotate_left
     · simp
-    · simp [hchans₁, ← hcondName, hlive_vars, SimR.varsToChans]
-      split <;> rename_i h
-      · have := hpath_conds_order _ _ _ h
-        omega
-      · split <;> rename_i h
-        · have := hpath_conds_order _ _ _ h
-          omega
-        · rfl
+    · simp [hchans₁, ← hcondName, hlive_vars, SimR.varsToChans,
+        path_conds_acyclic hpath_conds_order]
     replace ⟨pc₁, hpc₁, hsteps₁⟩ := exists_eq_left.mpr hsteps₁
     -- Step 2: Pop `switch_cond` and all live variable, and fire the `switch` operator
     have ⟨chans₂, hpop_switch_cond, hchans₂⟩ := pop_val_singleton _ _
@@ -120,24 +107,33 @@ theorem sim_step_br
         ∃ var,
           name = .var var ec.pathConds ∧
           ec.vars.getVar _ _ var = some val)
-      (by
-        simp [compileExpr.allVarsExcept, List.toVector]
-        apply List.Nodup.map
-        · simp [Function.Injective]
-        · exact List.Nodup.filter _ hdefined_vars_no_dup)
+      (allVarsExcept_nodup hdefined_vars_no_dup)
       (by
         intros name hname
         have ⟨var, hvar, hmem_var, hnot_mem_var⟩ := mem_allVarsExcept hname
-        simp at hnot_mem_var
-        simp [compileExpr.allVarsExcept, List.removeAll] at hname
-        simp [hchans₁, hchans₂, hpc₁, hvar, hnot_mem_var, ← hcondName, hlive_vars,
-          SimR.varsToChans, List.finIdxOf?, List.findFinIdx?, List.findFinIdx?.go]
+        simp only [List.mem_cons, List.not_mem_nil, or_false] at hnot_mem_var
+        simp only [List.removeAll, compileExpr.allVarsExcept, Vector.mem_map] at hname
         have ⟨_, h⟩ := (hdefined_vars var).mp hmem_var
-        simp [h])
+        simp [h, hchans₁, hchans₂, hpc₁, hvar, hnot_mem_var, ← hcondName, hlive_vars,
+          SimR.varsToChans, List.finIdxOf?, List.findFinIdx?, List.findFinIdx?.go])
+    have hchans₃_no_var {var pathConds} : chans₃ (.var var pathConds) = []
+    := by
+      simp [hchans₃, hchans₂, hchans₁, hpc₁, hlive_vars, ← hcondName,
+        SimR.varsToChans, VarMap.getVar, compileExpr.allVarsExcept, List.toVector,
+        List.finIdxOf?, List.findFinIdx?, List.findFinIdx?.go]
+      intros h₁ h₂ h₃
+      split
+      · rename_i h₄
+        have := (hdefined_vars var).mpr ⟨_, h₄⟩
+        if h₅ : var = cond then
+          simp [h₂ h₅ h₃]
+        else
+          simp [h₁ (List.mem_filter.mpr ⟨this, by simp [h₅]⟩) h₃.symm]
+      · rfl
     have hsteps₂ : Dataflow.Config.StepPlus _ _ _ _ pc _
       := Relation.TransGen.tail hsteps₁
           (Dataflow.Config.Step.step_switch
-            (by grind)
+            (by simp [hpc₁, hatoms, hrest, ← hcurrent])
             hpop_switch_cond
             hpop_all_vals
             hcondBool
@@ -145,198 +141,158 @@ theorem sim_step_br
             (inputs := compileExpr.allVarsExcept χ ec.definedVars [cond] ec.pathConds)
             (outputs₁ := compileExpr.allVarsExcept χ ec.definedVars [cond] leftConds)
             (outputs₂ := compileExpr.allVarsExcept χ ec.definedVars [cond] rightConds))
-    simp at hsteps₂
+    simp only at hsteps₂
     -- Simplify pushes
     rw [push_vals_empty] at hsteps₂
     rotate_left
-    · split
-      all_goals
-        simp [compileExpr.allVarsExcept, List.toVector]
-        apply List.Nodup.map
-        · simp [Function.Injective]
-        · exact List.Nodup.filter _ hdefined_vars_no_dup
+    · split <;> apply allVarsExcept_nodup hdefined_vars_no_dup
     · split
       all_goals
         intros name hname
-        simp [compileExpr.allVarsExcept] at hname
+        simp only [compileExpr.allVarsExcept, Vector.mem_map] at hname
         replace ⟨var, hvar, hname⟩ := hname
-        simp [List.toVector] at hvar
+        simp only [List.toVector, Vector.mem_mk, Array.mem_toArray] at hvar
         simp [hchans₁, hchans₂, hchans₃, hpc₁, ← hname,
           compileExpr.allVarsExcept, List.toVector,
           List.finIdxOf?, List.findFinIdx?, List.findFinIdx?.go,
           hlive_vars, SimR.varsToChans]
         intros h₁ _ h₂
-        have := h₁ hvar
-        simp [this h₂.symm]
-    simp at hsteps₂
+        exact False.elim (h₁ hvar h₂.symm)
+    have :
+      (if condBool = true then
+        compileExpr.allVarsExcept χ ec.definedVars [cond] leftConds
+      else
+        compileExpr.allVarsExcept χ ec.definedVars [cond] rightConds)
+      = compileExpr.allVarsExcept χ ec.definedVars [cond]
+        ((condBool, ChanName.var cond ec.pathConds) :: ec.pathConds)
+    := by
+      simp only [← hleftConds, ← hrightConds, ← hcondName]
+      cases condBool <;> simp
+    rw [this] at hsteps₂; clear this
     replace ⟨pc', hpc', hsteps₂⟩ := exists_eq_left.mpr hsteps₂
+    -- Prove simulation
     exists pc'
-    simp only [hsteps₂, true_and]
-    simp [hpc', hpc₁]
-    and_intros
-    · simp [heq_state]
-    · -- var to chans
-      funext name
-      simp [SimR.varsToChans]
-      cases name with
-      | var v pathConds =>
-        simp
-        have hchans₃_no_var: ∀ var pathConds,
-          chans₃ (.var var pathConds) = []
-        := by
-          intros var pathConds
-          simp [hchans₃, hchans₂, hchans₁, hpc₁, hlive_vars, ← hcondName,
-            SimR.varsToChans, VarMap.getVar, compileExpr.allVarsExcept, List.toVector,
-            List.finIdxOf?, List.findFinIdx?, List.findFinIdx?.go]
-          intros h₁ h₂ h₃
-          split
-          · rename_i h₄
-            have := (hdefined_vars var).mpr ⟨_, h₄⟩
-            if h₅ : var = cond then
-              simp [h₂ h₅ h₃]
-            else
-              simp [h₁ (List.mem_filter.mpr ⟨this, by simp [h₅]⟩) h₃.symm]
-          · rfl
-        have :
-          (if condBool = true then
-            compileExpr.allVarsExcept χ ec.definedVars [cond] leftConds
-          else
-            compileExpr.allVarsExcept χ ec.definedVars [cond] rightConds)
-          = compileExpr.allVarsExcept χ ec.definedVars [cond]
-          ((condBool, ChanName.var cond ec.pathConds) :: ec.pathConds)
-        := by
-          simp only [← hleftConds, ← hrightConds, ← hcondName]
-          cases condBool <;> simp
-        rw [this]
-        clear this
-        if h₁ : v = cond then
-          simp [h₁, compileExpr.allVarsExcept]
-          rw [Vector.finIdxOf?_eq_none_iff.mpr _]
-          · simp [VarMap.getVar, VarMap.removeVar, hchans₃, hchans₂, hpc₁, hchans₁,
+    constructor
+    · exact hsteps₂
+    · simp only [hpc', hpc₁]
+      and_intros
+      · simp [heq_state]
+      · funext name
+        simp only [SimR.varsToChans]
+        cases name with
+        | var v pathConds =>
+          simp
+          if h₁ : v = cond then
+            rw [allVarsExcept_finIdxOf?_none_if_removed (by simp [h₁])]
+            simp [h₁, VarMap.getVar, VarMap.removeVar, hchans₃, hchans₂, hpc₁, hchans₁,
               hlive_vars, SimR.varsToChans, ← hcondName,
               List.finIdxOf?, List.findFinIdx?, List.findFinIdx?.go]
-            intros
-            contradiction
-          · simp [List.toVector]
-            intros h₂
-            have := List.mem_filter.mp h₂
-            simp at this
-        else
-          if h₂ : v ∈ ec.definedVars then
-            simp [compileExpr.allVarsExcept]
-            split
-            · rename_i i h₃
-              simp at h₃
-              simp [List.toVector] at h₃
-              simp [h₃.1.2, Ne.symm h₁, VarMap.getVar, VarMap.removeVar]
-              have ⟨_, h₄⟩ := (hdefined_vars v).mp h₂
-              simp [VarMap.getVar] at h₄
-              have := List.forall₂_iff_get.mp hall_vals
-              have := this.2 i (by simp) (by simp)
-              simp [List.toVector, VarMap.getVar, compileExpr.allVarsExcept, h₃.1.1] at this
-              simp [this]
-            · simp [hchans₃_no_var]
-              rename_i h₃
-              have := Option.eq_none_iff_forall_ne_some.mpr h₃
-              simp at this
-              simp [List.toVector] at this
-              split
-              · have := this (List.mem_filter.mpr ⟨h₂, by simp [h₁]⟩)
-                intros h₅
-                simp [h₅] at this
-              · simp
+            intros _ h₂ h₃
+            exact False.elim (h₂ h₃)
           else
-            simp [compileExpr.allVarsExcept]
-            split
-            · rename_i i h₃
-              simp at h₃
-              simp [List.toVector] at h₃
-              have := List.get_mem (ec.definedVars.removeAll [cond]) i
-              simp [h₃.1.1] at this
-              have := List.mem_filter.mp this
-              simp [h₂ this.1]
-            · rename_i h₃
+            if h₂ : v ∈ ec.definedVars then
+              if h₃ : pathConds = (condBool, ChanName.var cond ec.pathConds) :: ec.pathConds then
+                have ⟨i, h₄⟩ := allVarsExcept_finIdxOf?_some (removedVars := [cond])
+                  h₂ (by simp [h₁]) h₃
+                simp [h₄]
+                simp [compileExpr.allVarsExcept] at h₄
+                simp [List.toVector] at h₄
+                simp [h₄.1.2, Ne.symm h₁, VarMap.getVar, VarMap.removeVar]
+                have ⟨_, h₅⟩ := (hdefined_vars v).mp h₂
+                simp only [VarMap.getVar] at h₅
+                have := List.forall₂_iff_get.mp hall_vals
+                have := this.2 i (by simp) (by simp)
+                simp [List.toVector, VarMap.getVar, compileExpr.allVarsExcept, h₄.1.1] at this
+                simp [this]
+              else
+                rw [allVarsExcept_finIdxOf?_none_if_diff_path_conds (by simp [Ne.symm h₃])]
+                simp [hchans₃_no_var, h₃]
+            else
+              rw [allVarsExcept_finIdxOf?_none_if_not_defined (by simp [h₂])]
               simp [hchans₃_no_var]
-              have := Option.eq_none_iff_forall_ne_some.mpr h₃
-              simp at this
-              simp [List.toVector] at this
               split
-              · rename_i h₄
-                simp [VarMap.getVar, VarMap.removeVar] at h₄
-                have := (hdefined_vars v).mpr ⟨_, h₄.2⟩
+              · rename_i h₃
+                simp [VarMap.getVar, VarMap.removeVar] at h₃
+                have := (hdefined_vars v).mpr ⟨_, h₃.2⟩
                 simp [h₂ this]
               · simp
-      | merge_cond name =>
-        simp [hchans₃, hchans₂, hpc₁, hchans₁,
-          compileExpr.allVarsExcept, List.finIdxOf?, List.findFinIdx?, List.findFinIdx?.go]
-        if h₁ : condName = name then
-          simp [h₁]
-          simp [hcondName, Eq.symm h₁]
-          have := instInterp.unique_toBool_fromBool _ _ hcondBool
-          if h₂ : condBool then
-            simp [h₂] at this ⊢
-            exact this
+        | merge_cond name =>
+          simp [hchans₃, hchans₂, hpc₁, hchans₁,
+            compileExpr.allVarsExcept, List.finIdxOf?, List.findFinIdx?, List.findFinIdx?.go]
+          if h₁ : condName = name then
+            simp [h₁]
+            simp [hcondName, Eq.symm h₁]
+            have := instInterp.unique_toBool_fromBool _ _ hcondBool
+            if h₂ : condBool then
+              simp [h₂] at this ⊢
+              exact this
+            else
+              simp [h₂] at this ⊢
+              split
+              · rename_i h
+                simp only [← hcondName] at h
+                have := hpath_conds_order _ _ _ h
+                omega
+              · simp [this]
           else
-            simp [h₂] at this ⊢
-            split
-            · rename_i h
-              simp only [← hcondName] at h
-              have := hpath_conds_order _ _ _ h
-              omega
-            · simp [this]
-        else
+            cases condBool
+            all_goals
+            simp [h₁]
+            simp [hcondName, Ne.symm h₁]
+            simp [← hcondName, hlive_vars, SimR.varsToChans]
+        | switch_cond name =>
           cases condBool
           all_goals
-          simp [h₁]
-          simp [hcondName, Ne.symm h₁]
-          simp [← hcondName, hlive_vars, SimR.varsToChans]
-      | switch_cond name =>
-        cases condBool
-        all_goals
-          simp [compileExpr.allVarsExcept, hchans₃, hchans₂, hpc₁, hchans₁]
-          intro h
-          simp [Ne.symm h, hlive_vars, SimR.varsToChans,
-            List.finIdxOf?, List.findFinIdx?, List.findFinIdx?.go]
-      | _ =>
-        cases condBool
-        all_goals
-          simp [compileExpr.allVarsExcept, hchans₃, hchans₂, hchans₁, hpc₁]
-          try rw [(Vector.finIdxOf?_eq_none_iff).mpr _]
-          simp [← hcondName, hlive_vars, hbr, SimR.varsToChans,
-            List.finIdxOf?, List.findFinIdx?, List.findFinIdx?.go]
-    · exact List.Nodup.filter _ hdefined_vars_no_dup
-    · simp; grind [VarMap.getVar, VarMap.removeVar]
-    · simp; grind
-    · simp; grind
-    · simp; grind
-    · simp only [hmerges]
-    · exact hwf_fn.1
-    · exact hwf_fn.2
-    · exists rest, carryInLoop
-      exists -- ctxLeft
-        if condBool then
-          ctxLeft ++ [
-            .fork condName #v[.switch_cond condName, .merge_cond condName],
-            .switch (.switch_cond condName)
-              (compileExpr.allVarsExcept χ ec.definedVars [cond] ec.pathConds)
-              (compileExpr.allVarsExcept χ ec.definedVars [cond] leftConds)
-              (compileExpr.allVarsExcept χ ec.definedVars [cond] rightConds)
-          ]
-        else
-          ctxLeft ++ [
-            .fork condName #v[.switch_cond condName, .merge_cond condName],
-            .switch (.switch_cond condName)
-              (compileExpr.allVarsExcept χ ec.definedVars [cond] ec.pathConds)
-              (compileExpr.allVarsExcept χ ec.definedVars [cond] leftConds)
-              (compileExpr.allVarsExcept χ ec.definedVars [cond] rightConds)
-          ] ++ compileExpr Op χ V S hnz (ec.definedVars.removeAll [cond]) leftConds left
-      exists -- ctxCurrent
-        if condBool then leftComp else rightComp
-      exists -- ctxRight
-        if condBool then
-          rightComp ++ [compileExpr.brMerge Op χ V m n condName ec.pathConds] ++ ctxRight
-        else
-          [compileExpr.brMerge Op χ V m n condName ec.pathConds] ++ ctxRight
-      grind
+            simp [compileExpr.allVarsExcept, hchans₃, hchans₂, hpc₁, hchans₁]
+            intro h
+            simp [Ne.symm h, hlive_vars, SimR.varsToChans,
+              List.finIdxOf?, List.findFinIdx?, List.findFinIdx?.go]
+        | _ =>
+          cases condBool
+          all_goals
+            simp [compileExpr.allVarsExcept, hchans₃, hchans₂, hchans₁, hpc₁]
+            try rw [(Vector.finIdxOf?_eq_none_iff).mpr _]
+            simp [← hcondName, hlive_vars, hbr, SimR.varsToChans,
+              List.finIdxOf?, List.findFinIdx?, List.findFinIdx?.go]
+      · exact List.Nodup.filter _ hdefined_vars_no_dup
+      · simp; grind [VarMap.getVar, VarMap.removeVar]
+      · simp; grind [SimR.OrderedPathConds]
+      · simp; grind [SimR.OrderedPathConds]
+      · simp; grind
+      · simp only [hmerges]
+      · exact hwf_fn.1
+      · exact hwf_fn.2
+      · simp
+        exists rest
+        simp only [hatoms, hcarryInLoop, hrest, List.append_assoc, hcomp_fn, true_and]
+        constructor
+        · exists -- ctxLeft
+            ctxLeft ++ if condBool then
+              [
+                .fork condName #v[.switch_cond condName, .merge_cond condName],
+                .switch (.switch_cond condName)
+                  (compileExpr.allVarsExcept χ ec.definedVars [cond] ec.pathConds)
+                  (compileExpr.allVarsExcept χ ec.definedVars [cond] leftConds)
+                  (compileExpr.allVarsExcept χ ec.definedVars [cond] rightConds)
+              ]
+            else
+              [
+                .fork condName #v[.switch_cond condName, .merge_cond condName],
+                .switch (.switch_cond condName)
+                  (compileExpr.allVarsExcept χ ec.definedVars [cond] ec.pathConds)
+                  (compileExpr.allVarsExcept χ ec.definedVars [cond] leftConds)
+                  (compileExpr.allVarsExcept χ ec.definedVars [cond] rightConds)
+              ] ++ leftComp
+          exists -- ctxRight
+            if condBool then
+              rightComp ++ [compileExpr.brMerge Op χ V m n condName ec.pathConds] ++ ctxRight
+            else
+              [compileExpr.brMerge Op χ V m n condName ec.pathConds] ++ ctxRight
+          split <;> rename_i h
+          · simp [h, ← hleftComp, ← hrightComp, ← hcurrent, ← hleftConds, ← hcondName]
+          · simp [h, ← hleftComp, ← hrightComp, ← hcurrent, ← hrightConds, ← hcondName]
+        · split
+          · exact hwf_left
+          · exact hwf_right
 
 end Wavelet.Simulation.Br
